first 6 even numbers + half the next even number:

1. 2 * 1 = 2
2. 2 * 2 = 4
3. 2 * 3 = 6
4. 2 * 4 = 8
5. 2 * 5 = 10
6. 2 * 6 = 12
7. 2 * 7 * 0.5 = 7

pattern:

2(sum of 1 to 6 ) + 7

let n = 6
sum of 1 to n = n(n+1)/2
then pattern is
2(n)(n+1)/2 + n + 1
n(n+1) + n + 1
n^2 +n + n + 1
n^2 + 2n + 1

n^2 + 2n + 1 = 465124
n^2 + 2n - 465123 = 0

quadratic formula
(-b ± sqrt(b^2 - 4ac)) / 2a

a = 1
b = 2
c = 465123

(-2 ± sqrt(4 + 1860492)) / 2
(-2 ± 1364) / 2

(-2 - 1364) / 2 = -683
(-2 + 1364) / 2 = 681
